src/Mman.fst
@@ -5,29 +5,115 @@ open Steel.Effect
 module A = Steel.Array
 
 module U8 = FStar.UInt8
+module U64 = FStar.UInt64
 module US = FStar.SizeT
-
-let array = Steel.ST.Array.array
-
-//noextract
-assume val mmap_init
-  (size: US.t)
-  : Steel (array U8.t)
-    emp
-    (fun r -> A.varray r)
-    (requires fun _ -> True)
-    (ensures fun _ ptr h1 ->
-      A.length ptr == US.v size /\
-      A.is_full_array ptr /\
-      A.asel ptr h1 == Seq.create (US.v size) U8.zero
-    )
-
-open NullOrVarray
+module AL = ArrayList
+module R = Steel.Reference
 
 open Utils2
 
+//TODO: TO BE REMOVED
+// only used during allocator initialization
+// checks that the return ptr is not null
+//assume val mmap_init
+//  (size: US.t)
+//  : Steel (array U8.t)
+//    emp
+//    (fun r -> A.varray r)
+//    (requires fun _ -> True)
+//    (ensures fun _ ptr h1 ->
+//      A.length ptr == US.v size /\
+//      A.is_full_array ptr /\
+//      A.asel ptr h1 == Seq.create (US.v size) U8.zero
+//    )
+
+/// 1) Initialization of the allocator
+// all functions with a _init suffix
+// are only meant to be used at initialization
+// and fail if the underlying mmap operation fails
+
+// mmap_u8_init returns a page-aligned array of bytes
+// that is, with an alignment of at least 16 bytes
+// hence the abstract property array_u8_proper_alignment here
+assume val mmap_u8_init (len: US.t)
+  : Steel (array U8.t)
+    emp
+    (fun a -> A.varray a)
+    (fun _ -> True)
+    (fun _ a h1 ->
+      A.length a == US.v len /\
+      A.is_full_array a /\
+      A.asel a h1 == Seq.create (US.v len) U8.zero /\
+      array_u8_proper_alignment a
+    )
+
+assume val mmap_u64_init (len: US.t)
+  : Steel (array U64.t)
+    emp
+    (fun a -> A.varray a)
+    (fun _ -> True)
+    (fun _ a h1 ->
+      A.length a == US.v len /\
+      A.is_full_array a /\
+      A.asel a h1 == Seq.create (US.v len) U64.zero
+    )
+
+assume val mmap_cell_status_init (len: US.t)
+  : Steel (array AL.cell)
+     emp
+    (fun a -> A.varray a)
+    (fun _ -> True)
+    (fun _ a h1 ->
+      A.length a == US.v len /\
+      A.is_full_array a
+    )
+
+assume val mmap_ptr_us_init (_:unit)
+  : SteelT (R.ref US.t)
+    emp
+    (fun r -> R.vptr r)
+
+module L = Steel.SpinLock
+
+open SizeClass
+noeq
+type size_class =
+  {
+    // The content of the sizeclass
+    data : size_class_struct;
+    // Mutex locking ownership of the sizeclass
+    lock : L.lock (size_class_vprop data);
+  }
+
+assume val mmap_sc_init (len: US.t)
+  : Steel (array size_class)
+     emp
+    (fun a -> A.varray a)
+    (fun _ -> True)
+    (fun _ a h1 ->
+      A.length a == US.v len /\
+      A.is_full_array a
+    )
+
+assume val mmap_sizes_init (len: US.t)
+  : Steel (array sc)
+     emp
+    (fun a -> A.varray a)
+    (fun _ -> True)
+    (fun _ a h1 ->
+      A.length a == US.v len /\
+      A.is_full_array a
+    )
+
+// used in src/LargeAlloc.fst
+// mmap_ptr_metadata
+
+/// 2) Large allocations wrappers
+
+open NullOrVarray
+
 //noextract
-assume val mmap_noinit
+assume val mmap_u8
   (size: US.t)
   : Steel (array U8.t)
     emp
@@ -39,6 +125,7 @@ assume val mmap_noinit
       not (A.is_null ptr) ==> (
         A.length ptr == US.v size /\
         A.is_full_array ptr /\
+        array_u8_proper_alignment ptr /\
         zf_u8 s
       )
     )
@@ -53,3 +140,4 @@ assume val munmap_u8 (ptr: array U8.t) (size: US.t)
       A.is_full_array ptr
     )
     (ensures fun _ _ _ -> True)
+
