src/SizeClass.fst
@@ -58,6 +58,7 @@ let slab_size : (v:US.t{US.v v == US.v metadata_max * U32.v page_size})
 
 type size_class_struct = s:size_class_struct'{
   A.length s.slab_region == US.v slab_size /\
+  array_u8_proper_alignment s.slab_region /\
   A.length s.md_bm_region == US.v metadata_max * 4 /\
   A.length s.md_region == US.v metadata_max
 }
@@ -133,6 +134,123 @@ let allocate_size_class_sl_lemma2
   )
   = ()
 
+#push-options "--fuel 0 --ifuel 0"
+let mod_arith_lemma
+  (n: nat) (k1 k2: pos)
+  : Lemma
+  (requires
+    k1 % k2 == 0 /\
+    k2 <= k1
+  )
+  (ensures
+    (n % k1) % k2 == n % k2
+  )
+  =
+  calc (==) {
+    ((n / k1) * k1) % k2;
+    == { Math.Lemmas.lemma_mod_mul_distr_r (n / k1) k1 k2 }
+    ((n / k1) * (k1 % k2)) % k2;
+    == { () }
+    0;
+  };
+  assert (((n / k1) * k1) % k2 == 0);
+  calc (==) {
+    (n % k1) % k2;
+    == { FStar.Math.Lemmas.euclidean_division_definition n k1 }
+    (n - (n / k1) * k1) % k2;
+    == { FStar.Math.Lemmas.lemma_mod_sub_distr n ((n / k1) * k1) k2 }
+    (n - ((n / k1) * k1) % k2) % k2;
+    == { () }
+    n % k2;
+  }
+
+let lemma_mod_plus2 (a k: int) (n: pos)
+  : Lemma
+  (requires
+    k % n == 0
+  )
+  (ensures
+    (a + k) % n == a % n
+  )
+  =
+  assert (k == k/n*n);
+  let k' = k/n in
+  Math.Lemmas.lemma_mod_plus a k' n
+
+let lemma_mod_mul2 (a k: int) (n: pos)
+  : Lemma
+  (requires
+    k % n == 0
+  )
+  (ensures
+    (a * k) % n == 0
+  )
+  =
+  Math.Lemmas.lemma_mod_mul_distr_r a k n
+
+let mod_arith_lemma_applied
+  (n: nat) (page_size sc align: pos)
+  : Lemma
+  (requires
+    sc % align == 0 /\
+    page_size % align == 0 /\
+    (n % page_size) % sc == 0 /\
+    align <= sc /\
+    sc <= page_size
+  )
+  (ensures n % align == 0)
+  =
+  Math.Lemmas.euclidean_division_definition n page_size;
+  assert (n % page_size == n - (n/page_size)*page_size);
+  let n' = n % page_size in
+  Math.Lemmas.euclidean_division_definition n' sc;
+  assert (n' % sc == n' - (n'/sc)*sc);
+  assert (n' % sc == 0);
+  assert (n' == n'/sc*sc);
+  assert (n - (n/page_size)*page_size == n'/sc*sc);
+  assert (n = (n/page_size)*page_size + n'/sc*sc);
+  lemma_mod_mul2 (n'/sc) sc align;
+  lemma_mod_plus2 ((n/page_size)*page_size) (n'/sc*sc) align;
+  assert (n % align = (n/page_size)*page_size % align);
+  lemma_mod_mul2 (n/page_size) page_size align;
+  lemma_mod_plus2 0 ((n/page_size)*page_size) align
+
+let allocate_size_class_aux
+  (scs: size_class_struct)
+  (r: array U8.t)
+  : Lemma
+  (requires
+    not (A.is_null r) ==> (
+      A.length r == U32.v scs.size /\
+      same_base_array r scs.slab_region /\
+      A.offset (A.ptr_of r) - A.offset (A.ptr_of scs.slab_region) >= 0 /\
+      ((A.offset (A.ptr_of r) - A.offset (A.ptr_of scs.slab_region)) % U32.v page_size) % (U32.v scs.size) == 0
+    )
+  )
+  (ensures
+    not (A.is_null r) ==> (
+      A.length r == U32.v scs.size /\
+      same_base_array r scs.slab_region /\
+      A.offset (A.ptr_of r) - A.offset (A.ptr_of scs.slab_region) >= 0 /\
+      ((A.offset (A.ptr_of r) - A.offset (A.ptr_of scs.slab_region)) % U32.v page_size) % (U32.v scs.size) == 0 /\
+      array_u8_proper_alignment r
+    )
+  )
+  =
+  if not (A.is_null r)
+  then (
+    assert (same_base_array r scs.slab_region);
+    assert (same_base_array scs.slab_region r);
+    assert (array_u8_proper_alignment scs.slab_region);
+    mod_arith_lemma_applied
+      (A.offset (A.ptr_of r) - A.offset (A.ptr_of scs.slab_region))
+      (U32.v page_size)
+      (U32.v scs.size)
+      16;
+    assert ((A.offset (A.ptr_of r) - A.offset (A.ptr_of scs.slab_region)) % 16 == 0);
+    array_u8_proper_alignment_lemma scs.slab_region r
+  ) else ()
+
 #push-options "--z3rlimit 100 --compat_pre_typed_indexed_effects"
 let allocate_size_class
   (scs: size_class_struct)
@@ -147,7 +265,8 @@ let allocate_size_class
       A.length r == U32.v scs.size /\
       same_base_array r scs.slab_region /\
       A.offset (A.ptr_of r) - A.offset (A.ptr_of scs.slab_region) >= 0 /\
-      ((A.offset (A.ptr_of r) - A.offset (A.ptr_of scs.slab_region)) % U32.v page_size) % (U32.v scs.size) == 0
+      ((A.offset (A.ptr_of r) - A.offset (A.ptr_of scs.slab_region)) % U32.v page_size) % (U32.v scs.size) == 0 /\
+      array_u8_proper_alignment r
     )
   )
   =
@@ -176,6 +295,7 @@ let allocate_size_class
     (size_class_vprop scs)
     (fun x y -> x == y)
     (fun m -> allocate_size_class_sl_lemma2 scs m);
+  allocate_size_class_aux scs result;
   return result
 
 open SlabsFree
